ctx: Prove all Context lemmas

Hybrid/Language/Context.lean
@@ -62,11 +62,12 @@ def from_index {φ : Form symbs s} {ψ : FormL symbs sorts} : Nat → Option (φ
   | 0   => sorry
   | n+1 => sorry
 
-def iso {φ : Form symbs s} {ψ : Form symbs s'} {χ τ : FormL symbs sorts} (C₁ : φ.Context χ) (C₂ : ψ.Context τ) : Prop :=
+def iso {φ : Form symbs s} {ψ : Form symbs s'} {χ : FormL symbs sorts} {τ : FormL symbs sorts'} (C₁ : φ.Context χ) (C₂ : ψ.Context τ) : Prop :=
   match C₁ with
   | .refl =>
       match C₂ with
       | .refl => True
+      | _ => False
   | .head =>
       match C₂ with
       | .head => True
@@ -76,21 +77,209 @@ def iso {φ : Form symbs s} {ψ : Form symbs s'} {χ τ : FormL symbs sorts} (C�
       | .tail ctx' => ctx.iso ctx'
       | _ => False
 
-lemma iso_trans {φ : Form symbs s} {ψ : Form symbs s'} {χ : Form symbs s''} {a b c : FormL symbs sorts} {C₁ : φ.Context a} {C₂ : ψ.Context b} {C₃ : χ.Context c} : C₁.iso C₂ → C₁.iso C₃ → C₂.iso C₃ := sorry
+@[refl]
+lemma iso_refl {φ : Form symbs s} {a : FormL symbs sorts} {C : φ.Context a} : C.iso C := by
+  induction C
+  . simp only [iso]
+  . simp only [iso]
+  . simp only [iso]
+    apply_assumption
 
-lemma if_iso {φ ψ : Form symbs s} {τ : FormL symbs sorts} (C₁ : φ.Context τ) (C₂ : ψ.Context τ) (h : C₁.iso C₂) : φ = ψ := sorry
+@[trans]
+lemma iso_trans {φ : Form symbs s} {ψ : Form symbs s'} {χ : Form symbs s''} {a b c : FormL symbs sorts} {C₁ : φ.Context a} {C₂ : ψ.Context b} {C₃ : χ.Context c} : C₁.iso C₂ → C₂.iso C₃ → C₁.iso C₃ := by
+  intro h1 h2
+  induction C₁
+  . cases C₂
+    . cases C₃
+      . simp only [iso]
+  . cases C₂
+    . cases C₃
+      . simp only [iso]
+      . simp only [iso] at h2
+    . cases C₃
+      . simp only [iso]
+      . simp only [iso] at h1
+  . cases C₂
+    . cases C₃
+      . simp only [iso] at h1
+      . simp only [iso] at h2
+    . cases C₃
+      . simp only [iso] at h2
+      . simp only [iso] at h2 h1 ⊢
+        apply_assumption
+        repeat assumption
 
-lemma if_iso_sorts {φ : Form symbs s} {ψ : Form symbs s'} {τ : FormL symbs sorts} (C₁ : φ.Context τ) (C₂ : ψ.Context τ) (h : C₁.iso C₂) : s = s' := sorry
+@[symm]
+lemma iso_symm {φ : Form symbs s} {ψ : Form symbs s'} {a b : FormL symbs sorts} {C₁ : φ.Context a} {C₂ : ψ.Context b} : C₁.iso C₂ → C₂.iso C₁ := by
+  intro h
+  induction C₁
+  . cases C₂
+    . simp only [iso]
+  . cases C₂
+    . simp only [iso]
+    . simp only [iso] at h
+  . cases C₂
+    . simp only [iso] at h
+    . simp only [iso] at h ⊢
+      apply_assumption
+      exact h
 
-lemma iso_subst {φ ψ χ : Form symbs s} {τ : FormL symbs sorts} {C₁ : φ.Context τ} {C₂ : ψ.Context C₁[χ]} (h : C₁.iso C₂) : ψ = χ := sorry
+lemma iso_trans' {φ : Form symbs s} {ψ : Form symbs s'} {χ : Form symbs s''} {a b c : FormL symbs sorts} {C₁ : φ.Context a} {C₂ : ψ.Context b} {C₃ : χ.Context c} : C₁.iso C₂ → C₁.iso C₃ → C₂.iso C₃ := by
+  intro h1 h2
+  apply iso_symm
+  apply iso_trans (iso_symm h2)
+  exact h1
 
-lemma iso_subst_sorts {φ χ : Form symbs s} {ψ : Form symbs s'} {τ : FormL symbs sorts} {C₁ : φ.Context τ} {C₂ : ψ.Context C₁[χ]} (h : C₁.iso C₂) : s = s' := sorry
+lemma if_iso {φ ψ : Form symbs s} {τ : FormL symbs sorts} (C₁ : φ.Context τ) (C₂ : ψ.Context τ) (h : C₁.iso C₂) : φ = ψ := by
+  induction τ with
+  | cons _ _ _ ih =>
+      cases C₁
+      . cases C₂
+        . rfl
+        . simp [iso] at h
+      . cases C₂
+        . simp [iso] at h
+        . rename_i ctx ctx'
+          apply ih ctx ctx'
+          exact h
+  | _ =>
+      cases C₁ with
+      | _ => cases C₂ with
+             | _ => rfl
 
-def subst_iso {φ ψ : Form symbs s} {χ : FormL symbs sorts} {C₁ : φ.Context χ} (C₂ : ψ.Context C₁[ψ]) (h : C₁.iso C₂) : (τ : Form symbs s) → Σ' C₃ : τ.Context C₁[τ], C₂.iso C₃ := sorry
+lemma if_iso_sorts {φ : Form symbs s} {ψ : Form symbs s'} {τ : FormL symbs sorts} (C₁ : φ.Context τ) (C₂ : ψ.Context τ) (h : C₁.iso C₂) : s = s' := by
+  induction τ with
+  | cons _ _ _ ih =>
+      cases C₁
+      . cases C₂
+        . rfl
+        . simp [iso] at h
+      . cases C₂
+        . simp [iso] at h
+        . rename_i ctx ctx'
+          apply ih ctx ctx'
+          exact h
+  | _ =>
+      cases C₁ with
+      | _ => cases C₂ with
+             | _ => rfl
 
-def subst_not_iso {φ χ : Form symbs s} {ψ : Form symbs s'} {τ : FormL symbs sorts} {C₁ : φ.Context τ} (C₂ : ψ.Context C₁[χ]) (h : ¬C₁.iso C₂) : (δ : Form symbs s) → Σ' C₃ : ψ.Context C₁[δ], C₂.iso C₃ := sorry
+lemma iso_subst {φ ψ χ : Form symbs s} {τ : FormL symbs sorts} {C₁ : φ.Context τ} {C₂ : ψ.Context C₁[χ]} (h : C₁.iso C₂) : ψ = χ := by
+  induction C₁
+  . cases C₂
+    . simp only [subst, id]
+  . cases C₂
+    . rfl
+    . simp only [iso] at h
+  . cases C₂
+    . simp only [iso] at h
+    . simp only [iso] at h
+      apply_assumption
+      exact h
 
-def subst_not_iso' {φ : Form symbs s} {ψ : Form symbs s'} {τ : FormL symbs sorts} {C₁ : φ.Context τ} (C₂ : ψ.Context τ) (h : ¬C₁.iso C₂) : (δ : Form symbs s) → Σ' C₃ : ψ.Context C₁[δ], C₂.iso C₃ := sorry
+lemma iso_subst_sorts {φ χ : Form symbs s} {ψ : Form symbs s'} {τ : FormL symbs sorts} {C₁ : φ.Context τ} {C₂ : ψ.Context C₁[χ]} (h : C₁.iso C₂) : s = s' := by
+  induction C₁
+  . cases C₂
+    . simp only
+  . cases C₂
+    . rfl
+    . simp only [iso] at h
+  . cases C₂
+    . simp only [iso] at h
+    . simp only [iso] at h
+      apply_assumption
+      exact h
+
+def subst_iso {φ ψ : Form symbs s} {χ : FormL symbs sorts} {C₁ : φ.Context χ} (C₂ : ψ.Context C₁[ψ]) (h : C₁.iso C₂) : (τ : Form symbs s) → Σ' C₃ : τ.Context C₁[τ], C₂.iso C₃ := λ τ => by
+  cases C₁
+  . cases C₂
+    . apply PSigma.mk
+      case fst =>
+        simp only [subst, id_eq]
+        exact refl
+      case snd =>
+        simp only [iso, id_eq]
+  . cases C₂
+    . apply PSigma.mk
+      case fst =>
+        simp only [subst]
+        exact head
+      case snd =>
+        simp only [iso, id_eq]
+    . simp only [iso] at h
+  . cases C₂
+    . simp only [iso] at h
+    case tail C' =>
+      simp only [iso] at h
+      have ⟨C'', iso⟩ := subst_iso C' h τ
+      apply PSigma.mk
+      case fst =>
+        simp only [subst]
+        exact tail C''
+      case snd =>
+        exact iso
+
+def subst_not_iso {φ : Form symbs s} {ψ : Form symbs s'} {τ : FormL symbs sorts} {C₁ : φ.Context τ} (C₂ : ψ.Context τ) (h : ¬C₁.iso C₂) : (δ : Form symbs s) → Σ' C₃ : ψ.Context C₁[δ], C₂.iso C₃ := λ δ => by
+  cases C₁
+  . cases C₂
+    . simp only [iso, not_true_eq_false] at h
+  . cases C₂
+    . simp only [iso, not_true_eq_false] at h
+    case tail C' =>
+      apply PSigma.mk
+      case fst =>
+        simp only [subst]
+        exact tail C'
+      case snd =>
+        simp only [iso, id_eq, iso_refl]
+  case tail C' =>
+    cases C₂
+    . simp only [subst]
+      apply PSigma.mk
+      case fst =>
+        exact head
+      case snd =>
+        simp only [iso]
+    case tail C'' =>
+      simp only [iso] at h
+      have ⟨C''', iso⟩ := subst_not_iso C'' h δ
+      apply PSigma.mk
+      case fst =>
+        simp only [subst]
+        exact tail C'''
+      case snd =>
+        exact iso
+
+def subst_not_iso' {φ χ : Form symbs s} {ψ : Form symbs s'} {τ : FormL symbs sorts} {C₁ : φ.Context τ} (C₂ : ψ.Context C₁[χ]) (h : ¬C₁.iso C₂) : (δ : Form symbs s) → Σ' C₃ : ψ.Context C₁[δ], C₂.iso C₃ := λ δ => by
+  cases C₁
+  . cases C₂
+    . simp only [iso, not_true_eq_false] at h
+  . cases C₂
+    . simp only [iso, not_true_eq_false] at h
+    case tail C' =>
+      apply PSigma.mk
+      case fst =>
+        simp only [subst]
+        exact tail C'
+      case snd =>
+        simp only [iso, id_eq, iso_refl]
+  case tail C' =>
+    cases C₂
+    . simp only [subst]
+      apply PSigma.mk
+      case fst =>
+        exact head
+      case snd =>
+        simp only [iso]
+    case tail C'' =>
+      simp only [iso] at h
+      have ⟨C''', iso⟩ := subst_not_iso' C'' h δ
+      apply PSigma.mk
+      case fst =>
+        simp only [subst]
+        exact tail C'''
+      case snd =>
+        exact iso
 
 /--
   Will be true if P is true for all other formulas in a FormL, with the exception of the one highlighted by the context.
@@ -116,6 +305,33 @@ def subst_to_ctx (χ : Form sig s)
           {φ : Form sig s}
           {ψ : FormL sig sorts}
           (C : Context φ ψ) :
-          χ.Context C[χ] := sorry
+          χ.Context C[χ] := by
+  cases ψ with
+  | cons χ χs =>
+      cases C
+      . exact Context.head
+      . apply Context.tail
+        apply subst_to_ctx
+  | _ =>
+      cases C
+      . exact Context.refl
+
+def subst_to_ctx_iso {χ : Form sig s}
+          {φ : Form sig s}
+          {ψ : FormL sig sorts}
+          (C : Context φ ψ) :
+          (χ.subst_to_ctx C).iso C := by
+  induction ψ with
+  | cons χ χs =>
+      cases C
+      . unfold subst_to_ctx
+        simp only [Context.iso]
+      . unfold subst_to_ctx
+        simp only [Context.iso]
+        apply_assumption
+  | _ =>
+      cases C
+      . unfold subst_to_ctx
+        simp only [Context.iso]
 
 end FormL
